<?xml version="1.0"?>


<!DOCTYPE rdf:RDF [
    <!ENTITY owl "http://www.w3.org/2002/07/owl#" >
    <!ENTITY xsd "http://www.w3.org/2001/XMLSchema#" >
    <!ENTITY rdfs "http://www.w3.org/2000/01/rdf-schema#" >
    <!ENTITY rdf "http://www.w3.org/1999/02/22-rdf-syntax-ns#" >
]>


<rdf:RDF xmlns="http://www.semanticweb.org/makdadmohamedyassine/ontologies/2025/1/untitled-ontology-5/"
     xml:base="http://www.semanticweb.org/makdadmohamedyassine/ontologies/2025/1/untitled-ontology-5/"
     xmlns:rdfs="http://www.w3.org/2000/01/rdf-schema#"
     xmlns:owl="http://www.w3.org/2002/07/owl#"
     xmlns:xsd="http://www.w3.org/2001/XMLSchema#"
     xmlns:rdf="http://www.w3.org/1999/02/22-rdf-syntax-ns#">
    <owl:Ontology rdf:about="http://www.semanticweb.org/makdadmohamedyassine/ontologies/2025/1/untitled-ontology-5">
        <rdfs:label xml:lang="en">Cannot Create Memento</rdfs:label>
        <rdfs:label xml:lang="en">Cannot Create Resource</rdfs:label>
        <rdfs:label xml:lang="en">Constraint Violation Exception</rdfs:label>
        <rdfs:label xml:lang="en">External Message Body Constraint</rdfs:label>
        <rdfs:label xml:lang="en">Incorrect Triple Subject Exception</rdfs:label>
        <rdfs:label xml:lang="en">Interaction Model Violation Exception</rdfs:label>
        <rdfs:label xml:lang="en">Invalid ACL Exception</rdfs:label>
        <rdfs:label xml:lang="en">Invalid Memento Path Exception</rdfs:label>
        <rdfs:label xml:lang="en">Malformed RDF Exception</rdfs:label>
        <rdfs:label xml:lang="en">Out Of Domain Subject Exception</rdfs:label>
        <rdfs:label xml:lang="en">Server Managed Property Exception</rdfs:label>
        <rdfs:label xml:lang="en">Server Managed Type Exception</rdfs:label>
        <rdfs:comment xml:lang="en">
          Fedora cannot handle versioning requests with a malformed memento ID.
          Memento ID is system generated, which is a timestamp in yyyyMMddHHmmss format.
        </rdfs:comment>
        <rdfs:comment xml:lang="en">Certain repository types can only be modified by the repository.</rdfs:comment>
        <rdfs:comment xml:lang="en">Fedora is unable to create the requested memento. Fedora does
        not support creating a memento with a Memento-Datetime header.
        </rdfs:comment>
        <rdfs:comment xml:lang="en">Fedora is unable to create the requested resource.  Fedora will
          not create a resource of type LDP Resource.  The type specified must be a subclass of
          LDP Resource.
        </rdfs:comment>
        <rdfs:comment xml:lang="en">Fedora wasn&apos;t able to create the LDPR with the specified LDP-RS as the ACL for one of the following reasons:
        the ACL URI in the link header does not exist, the ACL URI exists but does not contain a triple indicating rdf:type of http://fedora.info/definitions/v4/webac#Acl, or the ACL URI does not have the same domain as the LDPR.
        </rdfs:comment>
        <rdfs:comment xml:lang="en">Part of the request for creating/updating an External Message Body was missing
            or malformed. Link header must include a URI reference to an external resource from an allowed path;
            a link relation type (&apos;rel&apos;) that is set to &quot;http://fedora.info/definitions/fcrepo#ExternalContent&quot;;
            a &apos;handling&apos; attribute set to one of the following three values: proxy, redirect, or copy;
            and an optional &apos;type&apos; attribute representing the content type of the external body.
        </rdfs:comment>
        <rdfs:comment xml:lang="en">The RDF attempted to alter a property in the &lt;http://fedora.info/definitions/v4/repository#&gt; namespace. 
        These are system managed properties.</rdfs:comment>
        <rdfs:comment xml:lang="en">The RDF contained one or more triples where the subject was not contained inside
        the Fedora Repository. Fedora does not maintain RDF content about resources not contained within it.</rdfs:comment>
        <rdfs:comment xml:lang="en">The RDF contained one or more triples where the subject was not contained inside
        the resource being updated or created. RDF in Fedora is always an expression of the properties of a given
        resource.</rdfs:comment>
        <rdfs:comment xml:lang="en">The RDF violated Fedora&apos;s internal constraints to change the interaction model.</rdfs:comment>
        <rdfs:comment xml:lang="en">The RDF was incorrectly formed.  The response body from the failing request
        should offer useful information regarding the failure.</rdfs:comment>
        <rdfs:comment xml:lang="en">The request violated one of Fedora&apos;s internal constraints. Unfortunately we could not accurately determine which one.</rdfs:comment>
        <owl:imports rdf:resource="file:/home/makdadmohamedyassine/Downloads/fcrepo-webapp-6.4.0/static/constraints/static/constraints/CannotCreateMementoException"/>
        <owl:imports rdf:resource="file:/home/makdadmohamedyassine/Downloads/fcrepo-webapp-6.4.0/static/constraints/static/constraints/CannotCreateResourceWithAclException"/>
        <owl:imports rdf:resource="file:/home/makdadmohamedyassine/Downloads/fcrepo-webapp-6.4.0/static/constraints/static/constraints/ConstraintNotImplementedException"/>
        <owl:imports rdf:resource="file:/home/makdadmohamedyassine/Downloads/fcrepo-webapp-6.4.0/static/constraints/static/constraints/ConstraintViolationException"/>
        <owl:imports rdf:resource="file:/home/makdadmohamedyassine/Downloads/fcrepo-webapp-6.4.0/static/constraints/static/constraints/ExternalMessageBodyException"/>
        <owl:imports rdf:resource="file:/home/makdadmohamedyassine/Downloads/fcrepo-webapp-6.4.0/static/constraints/static/constraints/IncorrectTripleSubjectException"/>
        <owl:imports rdf:resource="file:/home/makdadmohamedyassine/Downloads/fcrepo-webapp-6.4.0/static/constraints/static/constraints/InteractionModelViolationException"/>
        <owl:imports rdf:resource="file:/home/makdadmohamedyassine/Downloads/fcrepo-webapp-6.4.0/static/constraints/static/constraints/InvalidACLException"/>
        <owl:imports rdf:resource="file:/home/makdadmohamedyassine/Downloads/fcrepo-webapp-6.4.0/static/constraints/static/constraints/InvalidMementoPathException"/>
        <owl:imports rdf:resource="file:/home/makdadmohamedyassine/Downloads/fcrepo-webapp-6.4.0/static/constraints/static/constraints/MalformedRdfException"/>
        <owl:imports rdf:resource="file:/home/makdadmohamedyassine/Downloads/fcrepo-webapp-6.4.0/static/constraints/static/constraints/OutOfDomainSubjectException"/>
        <owl:imports rdf:resource="file:/home/makdadmohamedyassine/Downloads/fcrepo-webapp-6.4.0/static/constraints/static/constraints/ServerManagedPropertyException"/>
        <owl:imports rdf:resource="file:/home/makdadmohamedyassine/Downloads/fcrepo-webapp-6.4.0/static/constraints/static/constraints/ServerManagedTypeException"/>
        <owl:imports rdf:resource="http://www.semanticweb.org/makdadmohamedyassine/ontologies/2025/1/untitled-ontology-5"/>
    </owl:Ontology>
    


    <!-- 
    ///////////////////////////////////////////////////////////////////////////////////////
    //
    // Annotation properties
    //
    ///////////////////////////////////////////////////////////////////////////////////////
     -->

    


    <!-- http://www.w3.org/2000/01/rdf-schema#comment -->

    <rdf:Description rdf:about="&rdfs;comment">
        <rdfs:isDefinedBy rdf:datatype="&xsd;Name"></rdfs:isDefinedBy>
        <rdfs:subPropertyOf rdf:resource="&rdfs;comment"/>
    </rdf:Description>
    


    <!-- http://www.w3.org/2000/01/rdf-schema#isDefinedBy -->

    <rdf:Description rdf:about="&rdfs;isDefinedBy">
        <rdfs:subPropertyOf rdf:resource="&rdfs;label"/>
        <rdfs:range rdf:resource="&xsd;Name"/>
        <rdfs:domain rdf:resource="&owl;Thing"/>
    </rdf:Description>
    


    <!-- http://www.w3.org/2000/01/rdf-schema#label -->

    <rdf:Description rdf:about="&rdfs;label">
        <rdfs:label>NEW VERSION</rdfs:label>
        <rdfs:domain rdf:resource="http://www.semanticweb.org/makdadmohamedyassine/ontologies/2025/1/untitled-ontology-5#NewThing"/>
    </rdf:Description>
    


    <!-- http://www.w3.org/2002/07/owl#backwardCompatibleWith -->

    <rdf:Description rdf:about="&owl;backwardCompatibleWith">
        <owl:priorVersion rdf:datatype="&xsd;anyURI">&lt;lyrasis&gt; LYRASIS &lt;\lyrasis&gt;</owl:priorVersion>
    </rdf:Description>
    


    <!-- http://www.w3.org/2002/07/owl#incompatibleWith -->

    <rdf:Description rdf:about="&owl;incompatibleWith">
        <rdfs:subPropertyOf rdf:resource="&owl;incompatibleWith"/>
    </rdf:Description>
    


    <!-- 
    ///////////////////////////////////////////////////////////////////////////////////////
    //
    // Object Properties
    //
    ///////////////////////////////////////////////////////////////////////////////////////
     -->

    


    <!-- http://www.semanticweb.org/makdadmohamedyassine/ontologies/2025/1/untitled-ontology-5#OWLObjectProperty_6cc758d1_bbff_464b_b688_33924ed4e7ba -->

    <owl:ObjectProperty rdf:about="http://www.semanticweb.org/makdadmohamedyassine/ontologies/2025/1/untitled-ontology-5#OWLObjectProperty_6cc758d1_bbff_464b_b688_33924ed4e7ba">
        <rdf:type rdf:resource="&owl;FunctionalProperty"/>
        <rdfs:isDefinedBy xml:lang="en">PrefixedName</rdfs:isDefinedBy>
        <rdfs:domain rdf:resource="http://www.semanticweb.org/makdadmohamedyassine/ontologies/2025/1/untitled-ontology-5#[Thing]_URN88e3e812_3fbb_4ac0_aa7a_dc82148d3830Trough"/>
    </owl:ObjectProperty>
    


    <!-- http://www.semanticweb.org/makdadmohamedyassine/ontologies/2025/1/untitled-ontology-5#ThingF -->

    <owl:ObjectProperty rdf:about="http://www.semanticweb.org/makdadmohamedyassine/ontologies/2025/1/untitled-ontology-5#ThingF">
        <rdf:type rdf:resource="&owl;TransitiveProperty"/>
        <rdfs:isDefinedBy></rdfs:isDefinedBy>
        <rdfs:subPropertyOf rdf:resource="http://www.semanticweb.org/makdadmohamedyassine/ontologies/2025/1/untitled-ontology-5#ThingF"/>
    </owl:ObjectProperty>
    


    <!-- 
    ///////////////////////////////////////////////////////////////////////////////////////
    //
    // Data properties
    //
    ///////////////////////////////////////////////////////////////////////////////////////
     -->

    


    <!-- http://www.semanticweb.org/makdadmohamedyassine/ontologies/2025/1/untitled-ontology-5#[InferedBy]_URN99e5a1b1_d19b_488c_b295_638f3c1f148dintoOnto -->

    <owl:DatatypeProperty rdf:about="http://www.semanticweb.org/makdadmohamedyassine/ontologies/2025/1/untitled-ontology-5#[InferedBy]_URN99e5a1b1_d19b_488c_b295_638f3c1f148dintoOnto">
        <rdfs:label xml:lang="fr">DataIS</rdfs:label>
        <rdfs:domain rdf:resource="http://www.semanticweb.org/makdadmohamedyassine/ontologies/2025/1/untitled-ontology-5#[Thing]_URN65765d9a_94de_43f2_bfef_7dab64a9eeaeTrough"/>
        <rdfs:seeAlso rdf:resource="&xsd;string"/>
        <rdfs:domain rdf:resource="&owl;Nothing"/>
        <owl:propertyDisjointWith rdf:resource="&owl;topDataProperty"/>
    </owl:DatatypeProperty>
    


    <!-- http://www.w3.org/2002/07/owl#topDataProperty -->

    <rdf:Description rdf:about="&owl;topDataProperty">
        <rdf:type rdf:resource="&owl;FunctionalProperty"/>
        <rdfs:subPropertyOf rdf:resource="http://www.semanticweb.org/makdadmohamedyassine/ontologies/2025/1/untitled-ontology-5#[InferedBy]_URN99e5a1b1_d19b_488c_b295_638f3c1f148dintoOnto"/>
    </rdf:Description>
    


    <!-- 
    ///////////////////////////////////////////////////////////////////////////////////////
    //
    // Classes
    //
    ///////////////////////////////////////////////////////////////////////////////////////
     -->

    


    <!-- http://www.semanticweb.org/makdadmohamedyassine/ontologies/2025/1/untitled-ontology-5#NewThing -->

    <owl:Class rdf:about="http://www.semanticweb.org/makdadmohamedyassine/ontologies/2025/1/untitled-ontology-5#NewThing">
        <owl:equivalentClass>
            <owl:Restriction>
                <owl:onProperty rdf:resource="&owl;topObjectProperty"/>
                <owl:allValuesFrom rdf:resource="http://www.semanticweb.org/makdadmohamedyassine/ontologies/2025/1/untitled-ontology-5#NewThing"/>
            </owl:Restriction>
        </owl:equivalentClass>
        <owl:disjointWith rdf:resource="&owl;Nothing"/>
    </owl:Class>
    


    <!-- http://www.semanticweb.org/makdadmohamedyassine/ontologies/2025/1/untitled-ontology-5#[InferedBy]_URN02709b60_822d_447d_bf41_5649e307b03bintoOnto -->

    <owl:Class rdf:about="http://www.semanticweb.org/makdadmohamedyassine/ontologies/2025/1/untitled-ontology-5#[InferedBy]_URN02709b60_822d_447d_bf41_5649e307b03bintoOnto">
        <rdfs:label xml:lang="fr">InferedBy</rdfs:label>
        <rdfs:subClassOf rdf:resource="http://www.semanticweb.org/makdadmohamedyassine/ontologies/2025/1/untitled-ontology-5#[Subject]_URN881bd07e_3747_4509_8f56_7e451929e264federated"/>
    </owl:Class>
    


    <!-- http://www.semanticweb.org/makdadmohamedyassine/ontologies/2025/1/untitled-ontology-5#[Subject]_URN881bd07e_3747_4509_8f56_7e451929e264federated -->

    <owl:Class rdf:about="http://www.semanticweb.org/makdadmohamedyassine/ontologies/2025/1/untitled-ontology-5#[Subject]_URN881bd07e_3747_4509_8f56_7e451929e264federated">
        <rdfs:label xml:lang="fr">Subject</rdfs:label>
    </owl:Class>
    


    <!-- http://www.semanticweb.org/makdadmohamedyassine/ontologies/2025/1/untitled-ontology-5#[Thing]_URN65765d9a_94de_43f2_bfef_7dab64a9eeaeTrough -->

    <owl:Class rdf:about="http://www.semanticweb.org/makdadmohamedyassine/ontologies/2025/1/untitled-ontology-5#[Thing]_URN65765d9a_94de_43f2_bfef_7dab64a9eeaeTrough">
        <rdfs:label xml:lang="fr">DOMOrigin</rdfs:label>
        <rdfs:subClassOf rdf:resource="http://www.semanticweb.org/makdadmohamedyassine/ontologies/2025/1/untitled-ontology-5#NewThing"/>
    </owl:Class>
    


    <!-- http://www.semanticweb.org/makdadmohamedyassine/ontologies/2025/1/untitled-ontology-5#[Thing]_URN88e3e812_3fbb_4ac0_aa7a_dc82148d3830Trough -->

    <owl:Class rdf:about="http://www.semanticweb.org/makdadmohamedyassine/ontologies/2025/1/untitled-ontology-5#[Thing]_URN88e3e812_3fbb_4ac0_aa7a_dc82148d3830Trough">
        <rdfs:label xml:lang="fr">DOMextension</rdfs:label>
        <rdfs:subClassOf rdf:resource="http://www.semanticweb.org/makdadmohamedyassine/ontologies/2025/1/untitled-ontology-5#fedoraThing"/>
    </owl:Class>
    


    <!-- http://www.semanticweb.org/makdadmohamedyassine/ontologies/2025/1/untitled-ontology-5#fedoraThing -->

    <owl:Class rdf:about="http://www.semanticweb.org/makdadmohamedyassine/ontologies/2025/1/untitled-ontology-5#fedoraThing">
        <rdfs:label></rdfs:label>
    </owl:Class>
    


    <!-- http://www.w3.org/2002/07/owl#Nothing -->

    <rdf:Description rdf:about="&owl;Nothing"/>
    


    <!-- http://www.w3.org/2002/07/owl#Thing -->

    <rdf:Description rdf:about="&owl;Thing">
        <owl:equivalentClass>
            <owl:Restriction>
                <owl:onProperty rdf:resource="http://www.semanticweb.org/makdadmohamedyassine/ontologies/2025/1/untitled-ontology-5#OWLObjectProperty_6cc758d1_bbff_464b_b688_33924ed4e7ba"/>
                <owl:cardinality rdf:datatype="&xsd;nonNegativeInteger">1</owl:cardinality>
            </owl:Restriction>
        </owl:equivalentClass>
    </rdf:Description>
    


    <!-- 
    ///////////////////////////////////////////////////////////////////////////////////////
    //
    // Individuals
    //
    ///////////////////////////////////////////////////////////////////////////////////////
     -->

    


    <!-- http://www.semanticweb.org/makdadmohamedyassine/ontologies/2025/1/untitled-ontology-5#OWLNamedIndividual_ec735cba_4a5d_4cdf_81ab_c7594bb5e347 -->

    <owl:NamedIndividual rdf:about="http://www.semanticweb.org/makdadmohamedyassine/ontologies/2025/1/untitled-ontology-5#OWLNamedIndividual_ec735cba_4a5d_4cdf_81ab_c7594bb5e347">
        <rdf:type rdf:resource="http://www.semanticweb.org/makdadmohamedyassine/ontologies/2025/1/untitled-ontology-5#NewThing"/>
        <rdf:type>
            <owl:Restriction>
                <owl:onProperty rdf:resource="&owl;topObjectProperty"/>
                <owl:someValuesFrom rdf:resource="http://www.semanticweb.org/makdadmohamedyassine/ontologies/2025/1/untitled-ontology-5#NewThing"/>
            </owl:Restriction>
        </rdf:type>
        <owl:topDataProperty rdf:datatype="&xsd;boolean">true</owl:topDataProperty>
        <rdfs:isDefinedBy xml:lang="en">BY_NAME</rdfs:isDefinedBy>
        <owl:sameAs rdf:resource="http://www.semanticweb.org/makdadmohamedyassine/ontologies/2025/1/untitled-ontology-5#reprise"/>
    </owl:NamedIndividual>
    


    <!-- http://www.semanticweb.org/makdadmohamedyassine/ontologies/2025/1/untitled-ontology-5#reprise -->

    <owl:Thing rdf:about="http://www.semanticweb.org/makdadmohamedyassine/ontologies/2025/1/untitled-ontology-5#reprise">
        <rdf:type rdf:resource="http://www.semanticweb.org/makdadmohamedyassine/ontologies/2025/1/untitled-ontology-5#fedoraThing"/>
        <rdf:type rdf:resource="&owl;NamedIndividual"/>
        <rdf:type>
            <owl:Restriction>
                <owl:onProperty rdf:resource="http://www.semanticweb.org/makdadmohamedyassine/ontologies/2025/1/untitled-ontology-5#ThingF"/>
                <owl:allValuesFrom rdf:resource="http://www.semanticweb.org/makdadmohamedyassine/ontologies/2025/1/untitled-ontology-5#fedoraThing"/>
            </owl:Restriction>
        </rdf:type>
        <owl:topDataProperty xml:lang="en">BY_NAME</owl:topDataProperty>
    </owl:Thing>
    <rdf:Description>
        <rdf:type>
            <owl:Restriction>
                <owl:onProperty rdf:resource="&owl;topObjectProperty"/>
                <owl:someValuesFrom rdf:resource="http://www.semanticweb.org/makdadmohamedyassine/ontologies/2025/1/untitled-ontology-5#NewThing"/>
            </owl:Restriction>
        </rdf:type>
        <owl:topDataProperty>geek bar</owl:topDataProperty>
    </rdf:Description>
    <rdf:Description>
        <owl:topDataProperty>FREEDOM</owl:topDataProperty>
    </rdf:Description>
    


    <!-- 
    ///////////////////////////////////////////////////////////////////////////////////////
    //
    // Annotations
    //
    ///////////////////////////////////////////////////////////////////////////////////////
     -->

    <rdf:Description rdf:about="&owl;versionInfo">
        <owl:backwardCompatibleWith>FEDORA COMMONS</owl:backwardCompatibleWith>
    </rdf:Description>
</rdf:RDF>



<!-- Generated by the OWL API (version 3.4.2) http://owlapi.sourceforge.net -->

